PhysLean/StringTheory/FTheory/SU5U1/Charges/PhenoConstrained/Elems/PhenoConstrained.lean
@@ -19,7 +19,6 @@ namespace SU5U1
 variable {I : CodimensionOneConfig}
 namespace Charges
 open PotentialTerm
-open ChargeProfile
 open CodimensionOneConfig
 open Tree
 
@@ -86,13 +85,13 @@ lemma not_isPhenoConstrained_of_mem_nonPhenoConstrainedCharges (I : CodimensionO
 set_option maxRecDepth 2500 in
 lemma isPresent_topYukawa_of_mem_nonPhenoConstrainedCharges_same :
     ∀ x ∈ (nonPhenoConstrainedCharges same).toMultiset,
-      IsPresent topYukawa (toChargeProfile topYukawa x) := by
+      IsPresent x topYukawa  := by
   intro x hx
   by_contra hnot
   have hx : x ∈ (nonPhenoConstrainedCharges same).toMultiset.filter
-      fun x => ¬ IsPresent topYukawa (toChargeProfile topYukawa x) := by
+      fun x => ¬ IsPresent x topYukawa := by
     simp_all
-  have hl : Multiset.filter (fun x => ¬ IsPresent topYukawa (toChargeProfile topYukawa x))
+  have hl : Multiset.filter (fun x => ¬ IsPresent x topYukawa)
     (nonPhenoConstrainedCharges same).toMultiset = ∅ := by rfl
   rw [hl] at hx
   simp at hx
@@ -100,13 +99,13 @@ lemma isPresent_topYukawa_of_mem_nonPhenoConstrainedCharges_same :
 set_option maxRecDepth 2000 in
 lemma isPresent_topYukawa_of_mem_nonPhenoConstrainedCharges_nearestNeighbor :
     ∀ x ∈ (nonPhenoConstrainedCharges nearestNeighbor).toMultiset,
-      IsPresent topYukawa (toChargeProfile topYukawa x) := by
+      IsPresent x topYukawa := by
   intro x hx
   by_contra hnot
   have hx : x ∈ (nonPhenoConstrainedCharges nearestNeighbor).toMultiset.filter
-      fun x => ¬ IsPresent topYukawa (toChargeProfile topYukawa x) := by
+      fun x => ¬ IsPresent x topYukawa := by
     simp_all
-  have hl : Multiset.filter (fun x => ¬ IsPresent topYukawa (toChargeProfile topYukawa x))
+  have hl : Multiset.filter (fun x => ¬ IsPresent x topYukawa)
     (nonPhenoConstrainedCharges nearestNeighbor).toMultiset = ∅ := by rfl
   rw [hl] at hx
   simp at hx
@@ -114,20 +113,20 @@ lemma isPresent_topYukawa_of_mem_nonPhenoConstrainedCharges_nearestNeighbor :
 set_option maxRecDepth 2000 in
 lemma isPresent_topYukawa_of_mem_nonPhenoConstrainedCharges_nextToNearestNeighbor :
     ∀ x ∈ (nonPhenoConstrainedCharges nextToNearestNeighbor).toMultiset,
-      IsPresent topYukawa (toChargeProfile topYukawa x) := by
+      IsPresent  x topYukawa := by
   intro x hx
   by_contra hnot
   have hx : x ∈ (nonPhenoConstrainedCharges nextToNearestNeighbor).toMultiset.filter
-      fun x => ¬ IsPresent topYukawa (toChargeProfile topYukawa x) := by
+      fun x => ¬ IsPresent  x topYukawa := by
     simp_all
-  have hl : Multiset.filter (fun x => ¬ IsPresent topYukawa (toChargeProfile topYukawa x))
+  have hl : Multiset.filter (fun x => ¬ IsPresent x topYukawa)
     (nonPhenoConstrainedCharges nextToNearestNeighbor).toMultiset = ∅ := by rfl
   rw [hl] at hx
   simp at hx
 
 lemma isPresent_topYukawa_of_mem_nonPhenoConstrainedCharges (I : CodimensionOneConfig) :
     ∀ x ∈ (nonPhenoConstrainedCharges I).toMultiset,
-      IsPresent topYukawa (toChargeProfile topYukawa x) :=
+      IsPresent x topYukawa :=
   match I with
   | same => isPresent_topYukawa_of_mem_nonPhenoConstrainedCharges_same
   | nearestNeighbor => isPresent_topYukawa_of_mem_nonPhenoConstrainedCharges_nearestNeighbor
