PhysLean/StringTheory/FTheory/SU5U1/Potential/Charges.lean
@@ -1,0 +1,501 @@
+/-
+Copyright (c) 2025 Joseph Tooby-Smith. All rights reserved.
+Released under Apache 2.0 license as described in the file LICENSE.
+Authors: Joseph Tooby-Smith
+-/
+import PhysLean.StringTheory.FTheory.SU5U1.Charges.Basic
+/-!
+
+# Charges associated with a potential term
+
+-/
+
+namespace FTheory
+namespace SU5U1
+
+namespace Charges
+
+def ofFieldKind (x : Charges) : FieldKinds → Finset ℤ
+  | .fiveBarHd => x.1.toFinset
+  | .fiveBarHu => x.2.1.toFinset
+  | .fiveBarMatter => x.2.2.1
+  | .tenMatter => x.2.2.2
+  | .fiveHd => x.1.toFinset.map ⟨Neg.neg, neg_injective⟩
+  | .fiveHu => x.2.1.toFinset.map ⟨Neg.neg, neg_injective⟩
+  | .fiveMatter => x.2.2.1.map ⟨Neg.neg, neg_injective⟩
+
+@[simp]
+lemma mem_ofFieldKind_fiveHd (x : ℤ) (y : Charges) :
+    x ∈ y.ofFieldKind FieldKinds.fiveHd ↔ -x ∈ y.ofFieldKind .fiveBarHd := by
+  simp [ofFieldKind, FieldKinds.fiveHd]
+  aesop
+
+@[simp]
+lemma mem_ofFieldKind_fiveHu (x : ℤ) (y : Charges) :
+    x ∈ y.ofFieldKind FieldKinds.fiveHu ↔ -x ∈ y.ofFieldKind .fiveBarHu := by
+  simp [ofFieldKind, FieldKinds.fiveHu]
+  aesop
+
+@[simp]
+lemma mem_ofFieldKind_fiveMatter (x : ℤ) (y : Charges) :
+    x ∈ y.ofFieldKind FieldKinds.fiveMatter ↔ -x ∈ y.ofFieldKind .fiveBarMatter := by
+  simp [ofFieldKind, FieldKinds.fiveBarHd]
+  aesop
+
+lemma ofFieldKind_subset_of_subset {x y : Charges} (h : x ⊆ y) (F : FieldKinds) :
+    x.ofFieldKind F ⊆ y.ofFieldKind F := by
+  rw [subset_def] at h
+  obtain ⟨h1, h2, h3, h4⟩ := h
+  cases F
+  all_goals simp_all [ofFieldKind]
+
+def ofPotentialTerm (x : Charges) (T : PotentialTerm) : Multiset ℤ :=
+  let add : Multiset ℤ → Multiset ℤ → Multiset ℤ := fun a b => (a.product b).map
+      fun (x, y) => x + y
+  (T.toFieldKinds.map fun F => (ofFieldKind x F).val).foldl add {0}
+
+
+lemma ofPotentialTerm_subset_of_subset {x y : Charges} (h : x ⊆ y) (T : PotentialTerm) :
+    x.ofPotentialTerm T ⊆ y.ofPotentialTerm T := by
+  have h1 {S1 S2 T1 T2 : Multiset ℤ} (h1 : S1 ⊆ S2) (h2 : T1 ⊆ T2) :
+      (S1.product T1) ⊆ S2.product T2 :=
+    Multiset.subset_iff.mpr (fun x => by simpa using fun h1' h2' => ⟨h1 h1', h2 h2'⟩)
+  rw [subset_def] at h
+  cases T
+  all_goals
+    simp [ofPotentialTerm, PotentialTerm.toFieldKinds]
+    repeat'
+      apply Multiset.map_subset_map <| Multiset.subset_iff.mpr <|
+        h1 _ (Finset.subset_def.mp (ofFieldKind_subset_of_subset h _))
+    simp
+
+def IsPresent  (x : Charges) (T : PotentialTerm) : Prop :=
+    0 ∈ ofPotentialTerm x T
+
+lemma isPresent_of_subset {T : PotentialTerm} {y x : Charges}
+    (h : y ⊆ x) (hy : y.IsPresent T) :
+    x.IsPresent T := ofPotentialTerm_subset_of_subset h T hy
+
+def isPresentForm (a b c : ℤ) : (T : PotentialTerm) → Charges
+  | .μ =>  (some a, some a, ∅ , ∅)
+  | .β =>  (none, some a, {a} , ∅)
+  | .Λ =>  (none, none, {a, b}, {- a - b})
+  | .W1 => (none, none, {- a - b - c}, {a, b, c})
+  | .W2 => (some (- a - b - c), none, ∅, {a, b, c})
+  | .W3 => (none, some (- a), {b, - b - 2 * a}, ∅)
+  | .W4 => (some (- c - 2 * b), some (- b), {c}, ∅)
+  | .K1 => (none, none, {-a}, {b, - a - b})
+  | .K2 => (some a, some b, ∅, {- a - b})
+  | .topYukawa => (none, some (-a), ∅, {b, - a - b})
+  | .bottomYukawa => (some a, none, {b}, {- a - b})
+
+lemma isPresentForm_isPresent {a b c : ℤ} {T : PotentialTerm} :
+    (isPresentForm a b c T).IsPresent T := by
+  simp [IsPresent, ofPotentialTerm, isPresentForm]
+  cases T
+  all_goals
+    simp [PotentialTerm.toFieldKinds, ofFieldKind, ofPotentialTerm]
+  any_goals omega
+  case' Λ =>
+    use a + b
+    simp
+    use a, b
+    simp
+    use 0, a
+    simp
+  case' W3 =>
+    use - 2 * a
+    apply And.intro ?_ (by omega)
+    use b, -b - 2 * a
+    apply And.intro ?_ (by omega)
+    simp
+    use 0, b
+    simp
+  case' K1 =>
+    use - a
+    apply And.intro ?_ (by omega)
+    use b, - a - b
+    apply And.intro ?_ (by omega)
+    simp
+    use 0, b
+    simp
+  case' topYukawa =>
+    use - a
+    apply And.intro ?_ (by omega)
+    use b, - a - b
+    apply And.intro ?_ (by omega)
+    simp
+    use 0, b
+    simp
+  case' W1 =>
+    use a + b + c
+    apply And.intro ?_ (by omega)
+    use a + b, c
+    apply And.intro ?_ (by omega)
+    simp
+    use a, b
+    simp
+    use 0, a
+    simp
+  case' W2 =>
+    use a + b + c
+    apply And.intro ?_ (by omega)
+    use a + b, c
+    apply And.intro ?_ (by omega)
+    simp
+    use a, b
+    simp
+    use 0, a
+    simp
+
+lemma isPresent_of_eq_isPresentForm {T : PotentialTerm}
+    (x : Charges) (h : ∃ a b c, x = isPresentForm a b c T) :
+    x.IsPresent T := by
+  obtain ⟨a, b, c, rfl⟩ := h
+  exact isPresentForm_isPresent
+open PotentialTerm in
+
+lemma isPresentForm_eq_of_subset {a b c a' b' c' : ℤ} {T : PotentialTerm}
+    (h : isPresentForm a b c T ⊆ isPresentForm a' b' c' T) (hT : T ≠ W1 ∧ T ≠ W2):
+    isPresentForm a b c T = isPresentForm a' b' c' T := by
+  cases T
+  case' W1 | W2 => simp at hT
+  all_goals
+    rw [subset_def] at h
+    simp [isPresentForm] at h ⊢
+  case' μ =>
+    subst h
+    rfl
+  case' β =>
+    subst h
+    rfl
+  case' K2 =>
+    obtain ⟨rfl, rfl, h2⟩ := h
+    rfl
+  case' W4 =>
+    obtain ⟨h2, rfl, rfl⟩ := h
+    rfl
+  case' bottomYukawa =>
+    obtain ⟨rfl, rfl, h2⟩ := h
+    rfl
+  case' Λ => obtain ⟨h2, h1⟩ := h
+  case' K1 =>  obtain ⟨rfl, h2⟩ := h
+  case' topYukawa => obtain ⟨rfl, h2⟩ := h
+  case' W3 => obtain ⟨rfl, h2⟩ := h
+  case' topYukawa | W3 | K1 | Λ  =>
+    rw [Finset.insert_subset_iff] at h2
+    simp at h2
+    obtain ⟨rfl | rfl , h1 | h2 ⟩ := h2
+    all_goals simp_all [Finset.pair_comm]
+
+
+lemma isPresentForm_card_le_degree {a b c : ℤ} {T : PotentialTerm} :
+    (isPresentForm a b c T).card ≤ T.degree := by
+  cases T
+  all_goals
+    simp [isPresentForm, PotentialTerm.toFieldKinds, ofFieldKind, ofPotentialTerm, card,
+      PotentialTerm.degree]
+  case' Λ =>
+    have h1 : Finset.card {a, b} ≤ 2 := Finset.card_le_two
+    omega
+  case' W3  =>
+    have h1 : Finset.card {b, -b - 2 * a} ≤ 2 := Finset.card_le_two
+    omega
+  case' K1  =>
+    have h1 : Finset.card {b, -a - b} ≤ 2 := Finset.card_le_two
+    omega
+  case' topYukawa  =>
+    have h1 : Finset.card {b, -a - b} ≤ 2 := Finset.card_le_two
+    omega
+  all_goals
+    have h1 : Finset.card {a, b, c} ≤ 3 := Finset.card_le_three
+    omega
+
+lemma isPresentForm_subset_isPresent_of_isPresent {T : PotentialTerm} {x : Charges}
+    (h : x.IsPresent T) :
+    ∃ a b c, isPresentForm a b c T ⊆ x ∧ (isPresentForm a b c T).IsPresent T := by
+  simp [IsPresent, ofPotentialTerm] at h
+  cases T
+  all_goals
+    simp [PotentialTerm.toFieldKinds] at h
+    obtain ⟨f1, f2, ⟨⟨f3, f4, ⟨h3, f4_mem⟩ , rfl⟩, f2_mem⟩, f1_add_f2_eq_zero⟩ := h
+  case' μ | β =>  obtain ⟨rfl⟩ := h3
+  case' Λ | W1 | W2 | W3 | W4 | K1 | K2 | topYukawa | bottomYukawa =>
+    obtain ⟨f5, f6, ⟨h4, f6_mem⟩, rfl⟩ := h3
+  case' Λ | K1 | K2 | topYukawa | bottomYukawa => obtain ⟨rfl⟩ := h4
+  case' W1 | W2 | W3 | W4 => obtain ⟨f7, f8, ⟨rfl, f8_mem⟩, rfl⟩ := h4
+  -- The cases which are present
+  case' μ => use f4, (f2), 0
+  case' β => use (- f4), f2, 0
+  case' Λ => use  f4, f6, f2
+  case' W1 => use  f4, f6, f8
+  case' W2 => use f4, f6, f8
+  case' W3 => use (f2), f6, f8
+  case' W4 => use f6, (f2), f8
+  case' K1 => use f2, f4, f6
+  case' K2 => use  f4, f6, f2
+  case' topYukawa => use (f2), f4, f6
+  case' bottomYukawa => use f2, f4, f6
+  all_goals
+    rw [subset_def]
+    simp_all [ofFieldKind, ofPotentialTerm, Finset.insert_subset_iff, isPresentForm]
+  all_goals
+    simp [IsPresent, ofPotentialTerm, PotentialTerm.toFieldKinds, ofFieldKind]
+  -- Replacements of equalities
+  case' W1 | W2 =>
+    have hf2 : f2 =  -f4 - f6 - f8 := by omega
+    subst hf2
+    simp_all
+  case' β =>
+    have hf2 : f4 = - f2 := by omega
+    subst hf2
+    simp_all
+  case' K2 =>
+    have hf2 : f2 = - f4 - f6 := by omega
+    subst hf2
+    simp_all
+  case' Λ =>
+    have hf2 : f2 = -f4 - f6 := by omega
+    subst hf2
+    simp_all
+  case' W3 =>
+    subst f4_mem
+    have hf8 : f8 = - f6 -2 * f4 := by omega
+    subst hf8
+    simp_all
+  case' bottomYukawa =>
+    have hf6 : f6 = - f2 - f4 := by omega
+    subst hf6
+    simp_all
+  -- IsPresent
+  any_goals omega
+  case' W3 =>
+    use (- f6 -2 * f4 ) + f6
+    apply And.intro ?_ (by omega)
+    try simp
+    use (- f6 -2 * f4 ), f6
+    simp
+    use 0, (- f6 -2 * f4 )
+    simp
+  case' W1 | W2   =>
+    use f8 + f6 + f4
+    apply And.intro ?_ (by omega)
+    use f8 + f6, f4
+  case' W1 | W2   =>
+    apply And.intro ?_ (by omega)
+    try simp
+    use f8, f6
+    simp
+    use 0, f8
+    simp
+  case' K1  =>
+    have hf6 : f6 = - f2 - f4 := by omega
+    subst hf6
+    simp_all
+    use (-f2 - f4) + f4
+    apply And.intro ?_ (by omega)
+    use (-f2 - f4), f4
+    apply And.intro ?_ (by omega)
+    simp
+    use 0, (-f2 - f4)
+    simp
+  case' topYukawa   =>
+    have hf2 : f2 = - f4 - f6 := by omega
+    subst hf2
+    simp_all
+  case' topYukawa | Λ  =>
+    use f6 + f4
+    apply And.intro ?_ (by omega)
+    use f6, f4
+    apply And.intro ?_ (by omega)
+    simp
+    use 0, f6
+    simp
+
+lemma subset_card_le_degree_isPresent_of_isPresent {T : PotentialTerm} {x : Charges}
+    (h : x.IsPresent T) : ∃ y ∈ x.powerset, y.card ≤ T.degree ∧ y.IsPresent T := by
+  obtain ⟨a, b, c, h1, h2⟩ := isPresentForm_subset_isPresent_of_isPresent h
+  use isPresentForm a b c T
+  simp_all
+  exact isPresentForm_card_le_degree
+
+/-!
+
+## Is Present decidable
+
+-/
+
+open PotentialTerm
+def IsPresentFast (y : Charges) (T : PotentialTerm)  : Prop :=
+  let qHd := y.1
+  let qHu := y.2.1
+  let Q5 := y.2.2.1
+  let Q10 := y.2.2.2
+  match T with
+  | μ => 0 ∈ (qHd.toFinset.product <| qHu.toFinset).val.map (fun x => x.1 - x.2)
+  | β => 0 ∈  (qHu.toFinset.product <| Q5).val.map (fun x => - x.1 + x.2)
+  | Λ => 0 ∈ (Q5.product <| Q5.product <| Q10).val.map (fun x => x.1 + x.2.1 + x.2.2)
+  | W1 => 0 ∈ (Q5.product <| Q10.product <| Q10.product <| Q10).val.map
+    (fun x => x.1 + x.2.1 + x.2.2.1 + x.2.2.2)
+  | W2 => 0 ∈ (qHd.toFinset.product <| Q10.product <| Q10.product <| Q10).val.map
+    (fun x => x.1 + x.2.1 + x.2.2.1 + x.2.2.2)
+  | W3 => 0 ∈ (qHu.toFinset.product <| Q5.product <| Q5).val.map
+    (fun x => -x.1 - x.1 + x.2.1 + x.2.2)
+  | W4 => 0 ∈ (qHd.toFinset.product <| qHu.toFinset.product <| Q5).val.map
+    (fun x => x.1 - x.2.1 - x.2.1 + x.2.2)
+  | K1 => 0 ∈ (Q5.product <| Q10.product <| Q10).val.map
+    (fun x => - x.1 + x.2.1 + x.2.2)
+  | K2 => 0 ∈  (qHd.toFinset.product <| qHu.toFinset.product <| Q10).val.map
+    (fun x => x.1 + x.2.1 + x.2.2)
+  | topYukawa => 0 ∈ (qHu.toFinset.product <| Q10.product <| Q10).val.map
+    (fun x => -x.1 + x.2.1 + x.2.2)
+  | bottomYukawa => 0 ∈ (qHd.toFinset.product <| Q5.product <| Q10).val.map
+    (fun x => x.1 + x.2.1 + x.2.2)
+
+lemma isPresentFast_of_isPresent {x : Charges} (T : PotentialTerm) (h : x.IsPresent T) :
+    x.IsPresentFast T := by
+  simp [IsPresent, ofPotentialTerm] at h
+  cases T
+  all_goals
+    simp [PotentialTerm.toFieldKinds] at h
+    obtain ⟨f1, f2, ⟨⟨f3, f4, ⟨h3, f4_mem⟩ , rfl⟩, f2_mem⟩, f1_add_f2_eq_zero⟩ := h
+  case' μ | β =>  obtain ⟨rfl⟩ := h3
+  case' Λ | W1 | W2 | W3 | W4 | K1 | K2 | topYukawa | bottomYukawa =>
+    obtain ⟨f5, f6, ⟨h4, f6_mem⟩, rfl⟩ := h3
+  case' Λ | K1 | K2 | topYukawa | bottomYukawa => obtain ⟨rfl⟩ := h4
+  case' W1 | W2 | W3 | W4 => obtain ⟨f7, f8, ⟨rfl, f8_mem⟩, rfl⟩ := h4
+  all_goals
+    simp [IsPresentFast]
+    simp only [SProd.sprod, Multiset.instSProd, Multiset.mem_product]
+    simp_all [ofFieldKind]
+  case' W1 => use f2, f4, f6, f8
+  case' W2 =>  use f2, f4, f6, f8
+  case' W3 =>  use (-f2), f6, f8
+  case' W4 => use f6, (-f4), f8
+  case' K1 => use (-f2), f4, f6
+  case' K2 => use f4, f6, f2
+  case' Λ => use f4, f6, f2
+  case' topYukawa => use (-f2), f4, f6
+  case' bottomYukawa => use f2, f4, f6
+  case' β => use (-f4), f2
+  all_goals simp_all
+  all_goals omega
+
+lemma isPresent_of_isPresentFast {x : Charges} (T : PotentialTerm) (h : x.IsPresentFast T) :
+    x.IsPresent T := by
+  cases T
+  all_goals
+    simp [IsPresentFast] at h
+    simp only [SProd.sprod, Multiset.instSProd, Multiset.mem_product] at h
+  case' μ | β =>
+    obtain ⟨q1, q2, ⟨q1_mem, q2_mem⟩, q_sum⟩ := h
+  case' Λ | W3 | W4 | K1 | K2 | topYukawa | bottomYukawa =>
+    obtain ⟨q1, q2, q3, ⟨q1_mem, q2_mem, q3_mem⟩, q_sum⟩ := h
+  case' W1 | W2 =>
+    obtain ⟨q1, q2, q3, q4, ⟨q1_mem, q2_mem, q3_mem, q4_mem⟩, q_sum⟩ := h
+  case' μ => refine isPresent_of_subset (y := (q1, q2, ∅, ∅)) ?μSub ?μP
+  case' β => refine isPresent_of_subset (y := (none, q1, {q2}, ∅)) ?βSub ?βP
+  case' Λ => refine isPresent_of_subset (y := (none, none, {q1, q2}, {q3})) ?ΛSub ?ΛP
+  case' W1 => refine isPresent_of_subset (y := (none, none, {q1}, {q2, q3, q4})) ?W1Sub ?W1P
+  case' W2 => refine isPresent_of_subset (y := (q1, none, ∅, {q2, q3, q4})) ?W2Sub ?W2P
+  case' W3 => refine isPresent_of_subset (y := (none, q1, {q2, q3}, ∅)) ?W3Sub ?W3P
+  case' W4 => refine isPresent_of_subset (y := (q1, q2, {q3}, ∅)) ?W4Sub ?W4P
+  case' K1 => refine isPresent_of_subset (y := (none, none, {q1}, {q2, q3})) ?K1Sub ?K1P
+  case' K2 => refine isPresent_of_subset (y := (q1, q2, ∅, {q3})) ?K2Sub ?K2P
+  case' topYukawa => refine isPresent_of_subset (y := (none, q1, ∅, {q2, q3})) ?topYukawaSub ?topYukawaP
+  case' bottomYukawa => refine isPresent_of_subset (y := (q1, none, {q2}, {q3})) ?bottomYukawaSub ?bottomYukawaP
+  case' μSub | βSub | ΛSub | W1Sub | W2Sub | W3Sub | W4Sub | K1Sub | K2Sub |
+      topYukawaSub | bottomYukawaSub =>
+    rw [subset_def]
+    simp_all [Finset.insert_subset]
+  all_goals
+    simp [IsPresent, ofPotentialTerm, PotentialTerm.toFieldKinds, ofFieldKind]
+  any_goals omega
+  case' ΛP =>
+    use - q3
+    simp
+    use - q1 - q3, q1
+    apply And.intro ?_ (by omega)
+    simp
+    use 0
+    simp
+    omega
+  case' W3P =>
+    use  2 * q1
+    apply And.intro ?_ (by omega)
+    use - q2 + 2 * q1, q2
+    apply And.intro ?_ (by omega)
+    simp
+    use 0, q3
+    simp
+    omega
+  case' K1P =>
+    use q1
+    apply And.intro ?_ (by omega)
+    use q1 - q2, q2
+    apply And.intro ?_ (by omega)
+    simp
+    use 0, q3
+    simp
+    omega
+  case' topYukawaP =>
+    use q1
+    apply And.intro ?_ (by omega)
+    use q1 - q2, q2
+    apply And.intro ?_ (by omega)
+    simp
+    use 0, q3
+    simp
+    omega
+  case' W1P | W2P =>
+    use - q1
+    apply And.intro ?_ (by omega)
+    use - q1 - q2, q2
+    apply And.intro ?_ (by omega)
+    simp
+    use -q1 - q2 - q3, q3
+    simp
+    use 0, q4
+    simp
+    omega
+
+lemma isPresent_iff_isPresentFast {x : Charges} {T : PotentialTerm} :
+    x.IsPresent T ↔ x.IsPresentFast T := by
+  constructor
+  · exact fun a => isPresentFast_of_isPresent T a
+  · exact fun a => isPresent_of_isPresentFast T a
+
+
+
+instance (x : Charges) (T : PotentialTerm) : Decidable (x.IsPresentFast T) :=
+  match T with
+  | μ => inferInstanceAs (Decidable (0 ∈ (x.1.toFinset.product <| x.2.1.toFinset).val.map (fun x => x.1 - x.2)))
+  | β => inferInstanceAs (Decidable (0 ∈ (x.2.1.toFinset.product <| x.2.2.1).val.map (fun x => - x.1 + x.2)))
+  | Λ => inferInstanceAs (Decidable (0 ∈ (x.2.2.1.product <| x.2.2.1.product <| x.2.2.2).val.map (fun x => x.1 + x.2.1 + x.2.2)))
+  | W1 => inferInstanceAs (Decidable (0 ∈ (x.2.2.1.product <| x.2.2.2.product <| x.2.2.2.product <| x.2.2.2).val.map
+      (fun x => x.1 + x.2.1 + x.2.2.1 + x.2.2.2)))
+  | W2 => inferInstanceAs (Decidable (0 ∈ (x.1.toFinset.product <| x.2.2.2.product <| x.2.2.2.product <| x.2.2.2).val.map
+      (fun x => x.1 + x.2.1 + x.2.2.1 + x.2.2.2)))
+  | W3 => inferInstanceAs (Decidable (0 ∈ (x.2.1.toFinset.product <| x.2.2.1.product <| x.2.2.1).val.map
+      (fun x => -x.1 - x.1 + x.2.1 + x.2.2)))
+  | W4 => inferInstanceAs (Decidable (0 ∈ (x.1.toFinset.product <| x.2.1.toFinset.product <| x.2.2.1).val.map
+      (fun x => x.1 - x.2.1 - x.2.1 + x.2.2)))
+  | K1 => inferInstanceAs (Decidable (0 ∈ (x.2.2.1.product <| x.2.2.2.product <| x.2.2.2).val.map
+      (fun x => - x.1 + x.2.1 + x.2.2)))
+  | K2 => inferInstanceAs (Decidable (0 ∈ (x.1.toFinset.product <| x.2.1.toFinset.product <| x.2.2.2).val.map
+      (fun x => x.1 + x.2.1 + x.2.2)))
+  | topYukawa => inferInstanceAs (Decidable (0 ∈ (x.2.1.toFinset.product <| x.2.2.2.product <| x.2.2.2).val.map
+      (fun x => -x.1 + x.2.1 + x.2.2)))
+  | bottomYukawa => inferInstanceAs (Decidable (0 ∈ (x.1.toFinset.product <| x.2.2.1.product <| x.2.2.2).val.map
+      (fun x => x.1 + x.2.1 + x.2.2)))
+
+
+
+instance (x : Charges) (T : PotentialTerm) : Decidable (x.IsPresent T) :=
+  decidable_of_iff (x.IsPresentFast T) isPresent_iff_isPresentFast.symm
+
+
+end Charges
+
+end SU5U1
+end FTheory
